Rename vars t/T to x/t

proof/Simple/EvJudge.v
@@ -6,20 +6,20 @@ Require Export SubstValueValue.
 (** Evaluation *******************************************)
 Inductive STEP : exp -> exp -> Prop :=
  |  EVLamApp
-    : forall T11 t12 tv2
-    ,  value tv2
-    -> STEP (XApp   (XLam T11 t12) tv2)
-            (subst tv2 t12)
+    : forall t11 x12 v2
+    ,  value v2
+    -> STEP (XApp   (XLam t11 x12) v2)
+            (subst v2 x12)
 
  |  EVApp1 
-    :  forall t1 t1' t2
-    ,  STEP t1 t1'
-    -> STEP (XApp t1 t2) (XApp t1' t2)
+    :  forall x1 x1' x2
+    ,  STEP x1 x1'
+    -> STEP (XApp x1 x2) (XApp x1' x2)
 
  |  EVApp2 
-    :  forall tv1 t2 t2'
-    ,  value tv1
-    -> STEP t2 t2'
-    -> STEP (XApp tv1 t2) (XApp tv1 t2').
+    :  forall v1 x2 x2'
+    ,  value v1
+    -> STEP x2 x2'
+    -> STEP (XApp v1 x2) (XApp v1 x2').
 
 Hint Constructors STEP.
